Playing with universes in SpecTree

state/SpecTree.fst
@@ -107,61 +107,114 @@ open FStar.Tactics.Typeclasses
 #set-options "--print_implicits --print_universes"
 
 noeq
-type pck_spec : Type u#(1 + (max a b)) =
-| SpecErr :
+type pck_spec =
+| SpecErr00 :
     bit:bool ->
-    argt:Type u#a ->
+    argt:Type u#0 ->
     wt_argt:witnessable argt ->
     pre:(argt -> st_pre) ->
-    rett:Type u#b ->
+    rett:Type u#0 ->
     wt_rett:witnessable rett ->
-    (post:(x:argt -> h0:heap -> st_post' u#b u#0 (resexn rett) (pre x h0))) ->
+    (post:(x:argt -> h0:heap -> st_post' (resexn rett) (pre x h0))) ->
     pck_spec
-| Spec :
+| SpecErr10 :
     bit:bool ->
-    argt:Type u#a ->
+    argt:Type u#1 ->
     wt_argt:witnessable argt ->
     pre:(argt -> st_pre) ->
-    rett:Type u#b ->
+    rett:Type u#0 ->
+    wt_rett:witnessable rett ->
+    (post:(x:argt -> h0:heap -> st_post' (resexn rett) (pre x h0))) ->
+    pck_spec
+| Spec00 :
+    bit:bool ->
+    argt:Type u#0 ->
+    wt_argt:witnessable argt ->
+    pre:(argt -> st_pre) ->
+    rett:Type u#0 ->
     wt_rett:witnessable rett ->
     (post:(x:argt -> h0:heap -> st_post' rett (pre x h0))) ->
     pck_spec
 
+let argt0 (p:pck_spec{Spec00? p \/ SpecErr00? p}) : Type u#0 =
+  match p with
+  | SpecErr00 _ argt _ _ _ _ _ -> argt
+  | Spec00 _ argt _ _ _ _ _ -> argt
+
+let wt_argt0 (p:pck_spec{Spec00? p \/ SpecErr00? p}) : witnessable (argt0 p) =
+  match p with
+  | SpecErr00 _ _ wt _ _ _ _ -> wt
+  | Spec00 _ _ wt _ _ _ _ -> wt
+
+let argt1 (p:pck_spec{SpecErr10? p}) : Type u#1 =
+  match p with
+  | SpecErr10 _ argt _ _ _ _ _ -> argt  
+
+let rett0 (p:pck_spec) : Type u#0 =
+  match p with
+  | SpecErr00 _ _ _ _ rett _ _ -> rett
+  | Spec00 _ _ _ _ rett _ _ -> rett
+  | SpecErr10 _ _ _ _ rett _ _ -> rett
+
+let wt_rett0 (p:pck_spec) : witnessable (rett0 p) =
+  match p with
+  | SpecErr00 _ _ _ _ _ wt _ -> wt
+  | Spec00 _ _ _ _ _ wt _ -> wt
+  | SpecErr10 _ _ _ _ _ wt _ -> wt
+
+let bit (p:pck_spec) : bool =
+  match p with
+  | SpecErr00 b _ _ _ _ _ _ -> b
+  | SpecErr10 b _ _ _ _ _ _ -> b
+  | Spec00 b _ _ _ _ _ _ -> b
+
+let pre0 (p:pck_spec{Spec00? p \/ SpecErr00? p}) : argt0 p -> st_pre =
+  match p with
+  | SpecErr00 _ _ _ pre _ _ _ -> pre
+  | Spec00 _ _ _ pre _ _ _ -> pre
+
 noeq
 type hoc a3p : (s:pck_spec) -> Type =
 | TrivialPre :
-    #s:pck_spec{Spec? s /\ Spec?.bit s == true} ->
-    c_pre:(x:(Spec?.argt s) -> Lemma (forall h0. pre_poly_arrow a3p #(Spec?.argt s) #(Spec?.wt_argt s) x h0 ==> (Spec?.pre s) x h0)) ->
-    c_post:(x:(Spec?.argt s) -> r:(Spec?.rett s) -> Lemma (forall h0 h1. (Spec?.post s) x h0 r h1 ==> post_poly_arrow a3p #(Spec?.rett s) #(Spec?.wt_rett s) h0 r h1))
+    #s:pck_spec{Spec00? s /\ bit s == true} ->
+    c_pre:(x:(argt0 s) -> 
+        Lemma (forall h0. pre_poly_arrow a3p #(argt0 s) #(wt_argt0 s) x h0 ==> (pre0 s) x h0)) ->
+    c_post:(x:(argt0 s) -> r:(rett0 s) -> 
+        Lemma (forall h0 h1. (Spec00?.post s) x h0 r h1 ==> post_poly_arrow a3p #(rett0 s) #(wt_rett0 s) h0 r h1))
     -> hoc a3p s
 
 | TrivialPost :
-    #s:pck_spec{Spec? s /\ Spec?.bit s == false} ->
-    c_pre:(x:(Spec?.argt s) -> Lemma (forall h0. (Spec?.pre s) x h0 ==> pre_poly_arrow a3p #(Spec?.argt s) #(Spec?.wt_argt s) x h0)) ->
-    c_post:(x:(Spec?.argt s) -> r:(Spec?.rett s) -> Lemma (forall h0 h1. post_poly_arrow a3p #(Spec?.rett s) #(Spec?.wt_rett s) h0 r h1 ==> (Spec?.post s) x h0 r h1))
+    #s:pck_spec{Spec00? s /\ bit s == false} ->
+    c_pre:(x:(argt0 s) ->
+        Lemma (forall h0. (pre0 s) x h0 ==> pre_poly_arrow a3p #(argt0 s) #(wt_argt0 s) x h0)) ->
+    c_post:(x:(argt0 s) -> r:(rett0 s) -> 
+        Lemma (forall h0 h1. post_poly_arrow a3p #(rett0 s) #(wt_rett0 s) h0 r h1 ==> (Spec00?.post s) x h0 r h1))
     -> hoc a3p s
 
 | EnforcePre :
-    #s:pck_spec{SpecErr? s /\ SpecErr?.bit s == true} ->
-    check:(select_check a3p (SpecErr?.argt s) unit
-                        (pre_poly_arrow a3p #(SpecErr?.argt s) #(SpecErr?.wt_argt s))
-                        (fun x _ _ h1 -> (SpecErr?.pre s) x h1)) ->
-    c_post:(x:(SpecErr?.argt s) -> r:(resexn (SpecErr?.rett s)) -> Lemma (forall h0 h1. (SpecErr?.post s) x h0 r h1 ==> post_poly_arrow a3p #(resexn (SpecErr?.rett s)) #(witnessable_resexn _ #(SpecErr?.wt_rett s)) h0 r h1))
+    #s:pck_spec{SpecErr00? s /\ bit s == true} ->
+    check:(select_check a3p (argt0 s) unit
+                        (pre_poly_arrow a3p #(argt0 s) #(wt_argt0 s))
+                        (fun x _ _ h1 -> (pre0 s) x h1)) ->
+    c_post:(x:(argt0 s) -> r:(resexn (rett0 s)) -> 
+        Lemma (forall h0 h1. (SpecErr00?.post s) x h0 r h1 ==> post_poly_arrow a3p #(resexn (rett0 s)) #(witnessable_resexn _ #(wt_rett0 s)) h0 r h1))
     -> hoc a3p s
 
 | EnforcePost :
-    #s:pck_spec{SpecErr? s /\ SpecErr?.bit s == false} ->
-    c_pre:(x:(SpecErr?.argt s) -> Lemma (forall h0. (SpecErr?.pre s) x h0 ==> pre_poly_arrow a3p #(SpecErr?.argt s) #(SpecErr?.wt_argt s) x h0)) ->
-    c_post:(x:(SpecErr?.argt s) -> e:err -> Lemma (forall h0 h1. (SpecErr?.pre s) x h0 /\ post_poly_arrow a3p #_ #(witnessable_resexn _ #(SpecErr?.wt_rett s)) h0 (Inr e) h1 ==> (SpecErr?.post s) x h0 (Inr e) h1)) ->
-    check:(select_check a3p (SpecErr?.argt s) (resexn (SpecErr?.rett s)) #(witnessable_resexn _ #(SpecErr?.wt_rett s)) (SpecErr?.pre s) (SpecErr?.post s))
+    #s:pck_spec{SpecErr00? s /\ bit s == false} ->
+    c_pre:(x:(argt0 s) -> 
+        Lemma (forall h0. (pre0 s) x h0 ==> pre_poly_arrow a3p #(argt0 s) #(wt_argt0 s) x h0)) ->
+    c_post:(x:(argt0 s) -> e:err -> 
+        Lemma (forall h0 h1. (pre0 s) x h0 /\ post_poly_arrow a3p #_ #(witnessable_resexn _ #(wt_rett0 s)) h0 (Inr e) h1 ==> (SpecErr00?.post s) x h0 (Inr e) h1)) ->
+    check:(select_check a3p (argt0 s) (resexn (rett0 s)) #(witnessable_resexn _ #(wt_rett0 s)) (pre0 s) (SpecErr00?.post s))
     -> hoc a3p s
 
-type pck_hoc a3p : Type u#(1+(max a b))=
+type pck_hoc a3p : Type =
   s:pck_spec & (hoc a3p s)
 
 private
 let myspec : pck_spec =
-  SpecErr
+  SpecErr00
     true
     (ref int)
     (witnessable_ref int)
@@ -173,10 +226,10 @@ let myspec : pck_spec =
 private
 let test_pre : hoc c3p myspec =
   EnforcePre
-    (fun (x:(SpecErr?.argt myspec)) ->
+    (fun (x:(argt0 myspec)) ->
       let x : ref int = x in
       let eh0 = get_heap () in
-      let check : cb_check c3p (ref int) unit (pre_poly_arrow c3p #(SpecErr?.argt myspec) #(SpecErr?.wt_argt myspec)) (fun x _ _ h1 -> (SpecErr?.pre myspec) x h1) x eh0 = (
+      let check : cb_check c3p (ref int) unit (pre_poly_arrow c3p #(argt0 myspec) #(wt_argt0 myspec)) (fun x _ _ h1 -> (pre0 myspec) x h1) x eh0 = (
         fun _ ->
           assert (witnessed (contains_pred x));
           recall (contains_pred x);
@@ -188,7 +241,7 @@ let test_pre : hoc c3p myspec =
 
 private
 let myspec' : pck_spec =
-  SpecErr
+  SpecErr00
     false
     (ref int)
     (witnessable_ref int)
@@ -205,7 +258,7 @@ let test_post : hoc c3p myspec' =
     (fun x ->
       let x : ref int = x in
       let eh0 = get_heap () in
-      let check : cb_check c3p (ref int) (resexn unit) #(witnessable_resexn _ #(SpecErr?.wt_rett myspec')) (SpecErr?.pre myspec') (SpecErr?.post myspec') x eh0 = (
+      let check : cb_check c3p (ref int) (resexn unit) #(witnessable_resexn _ #(wt_rett0 myspec')) (pre0 myspec') (SpecErr00?.post myspec') x eh0 = (
         fun _ ->
           assert (witnessed (contains_pred x));
           recall (contains_pred x);
@@ -214,7 +267,7 @@ let test_post : hoc c3p myspec' =
       ) in
       (| eh0, check |))
 
-type spec_tree : Type u#(1 + (max a b)) = tree pck_spec
+type spec_tree : Type = tree pck_spec
 
-let hoc_tree a3p (st:spec_tree) : Type u#(1 + (max a b)) =
+let hoc_tree a3p (st:spec_tree) : Type =
   hocs:(tree (pck_hoc a3p)){equal_trees st (map_tree hocs dfst)}
